Debt_Axiom/Debt_Axiom.thy
@@ -1,0 +1,17 @@
+theory Debt_Axiom
+  imports Pure
+  keywords "debt_axiomatization"  :: thy_stmt
+    and    "discharge_debt_axiom" :: thy_decl
+    and    "print_debt_axiom"     :: diag
+    and "unspecified_type" :: thy_decl
+    and "specify_type"     :: thy_decl
+    and "morphisms"        :: quasi_command
+begin
+
+declare [ [ML_debugger, ML_exception_debugger] ]
+
+ML_file \<open>kernel-sig.ML\<close>
+ML_file \<open>kernel.ML\<close> \<comment> \<open>the only kernel, consisting of 28 lines of ML excluding blanks\<close>
+ML_file \<open>Debt_Axiom.ML\<close>
+
+end
