Debt_Axiom/example/Debt_Axiom_Doc.thy
@@ -1,0 +1,127 @@
+theory Debt_Axiom_Doc
+  imports Main Debt_Axiom.Debt_Axiom
+begin
+
+section \<open>Introduction over an Example\<close>
+
+text \<open>Debt Axiom provides an approach to safely declare an axiom early, build anything above
+  the axiom, and later prove the validity of the previously declared axiom.
+  The declared axioms are not free, but require certificates later.
+  They are recorded in a ledger so we name them, \<^emph>\<open>debt axioms\<close>.
+  A ML kernel validates the certificate and especially it does not depend on
+  any declared debt axioms, so the certification is valid and it is a safe way to declare axioms.
+  The ML kernel is tiny, consisting of 28 lines of code only, and depending only on
+  Isabelle's kernel.
+
+  It resembles Locale which enables local assumptions, but we do not use locales and they are
+  real axioms, so we circumvent the limitations of Locale like incomplete supports for some
+  Isabelle functions like syntax translation, and complexity of multi-dependence especially
+  when the hierarchy is complicated, and also performance cost during activating a huge locale
+  when using @{command context} command and \<open>(in locale)\<close> syntax.
+
+  An example usage of the library is building an extensible modular semantic library, where
+  we pre-build small snippets each of which formalizes a specific semantic feature,
+  and we assemble the snippets of all the semantic features of a target language
+  when we are going to formalize it.
+  Each snippet can be an Isabelle theory and in the final assembly we import only the features that
+  the target language needs.
+
+  If we follow a deep embedding approach where two semantic types are used to model the type
+    and the value of the language respectively, note,
+  in such a generic library supporting free plug-in of various semantic features,
+  the actual definition of the semantic types cannot be decided until the final target language
+  to be formalized is given, because the complete semantic features are not decided until
+  that time.
+
+
+  However, if we want the library to be really useful by providing some reasoning supports and
+    automatic mechanisms, we do need first the declarations of the semantic types,
+    and partial definition about the semantic feature concerned by the module,
+    so that we can provide some mechanisms for the feature.
+
+  The Debt Axiom package addresses 
+  The tour starts from declaring semantic types used in our library to model the type
+    and the value of the language respectively.
+  
+  Therefore, we just \<^emph>\<open>declare\<close> the types in an \<^emph>\<open>unspecified\<close> way.
+\<close>
+
+unspecified_type VAL
+
+text \<open>They are unspecified meaning they are just declared but not finally defined.
+The definition can be given later after the final target language is given and decides
+the complete target semantic features.
+
+We continue declare some basic infrastructure in the formalization.
+\<open>typ_of\<close> give the type of a 
+\<close>
+
+
+text \<open>Then we build a semantic module for integer value and its arithmetic.
+In a new theory file for this feature, we declare the constructor of the integer model and also
+its destructor.
+\<close>
+
+debt_axiomatization mk_int :: \<open>int \<Rightarrow> VAL\<close>
+               and dest_int :: \<open>VAL \<Rightarrow> int\<close>
+              where mk_int_inj[simp]: \<open>dest_int (mk_int i) = i\<close>
+
+text \<open>\<open>dest_int\<close> should be the inverse function of \<open>mk_int\<close>. We declare this property by a debt
+  axiom, and require the final semantic assembly to discharge the proof of the axiom.
+  The @{command print_debt_axiom} now lists \<open>dest_int\<close> as an obligation debt.
+\<close>
+
+print_debt_axiom
+  \<comment> \<open>\<open>\<And>i. dest_int (mk_int i) = i\<close>\<close>
+
+text \<open>Formalization of instructions and various automation can be built above the semantic models.\<close>
+
+definition \<open>op_add va vb = mk_int (dest_int va + dest_int vb)\<close>
+
+lemma \<open>op_add (mk_int (1::int)) (op_add (mk_int 2) (mk_int 3)) = mk_int 6\<close>
+  unfolding op_add_def by simp
+
+text \<open>Meantime, we may formalize array in another theory file.\<close>
+
+debt_axiomatization mk_array :: \<open>VAL list \<Rightarrow> VAL\<close>
+              and dest_array :: \<open>VAL \<Rightarrow> VAL list\<close>
+  where mk_array_inj[simp]: \<open>dest_array (mk_array x) = x\<close>
+
+definition \<open>op_push v vL = mk_array (v # dest_array vL)\<close>
+definition \<open>op_peek vL = hd (dest_array vL)\<close>
+definition \<open>op_pop  vL = mk_array (tl (dest_array vL))\<close>
+
+lemma \<open>op_peek (op_push v L) = v\<close>
+  unfolding op_peek_def op_push_def by simp
+
+text \<open>Now in the final theory file assembling the semantic modules,
+  we instantiate the unspecified constants and discharge the debt axioms.\<close>
+
+datatype val = V_int (dest_V_int: int) | V_array (dest_V_array: \<open>val list\<close>)
+
+specify_type VAL[simp]: VAL = val
+
+print_debt_axiom  
+
+specification (mk_int dest_int mk_array dest_array)
+  mk_int_def': \<open>mk_int = VAL.inj o V_int\<close>
+  dest_int_def': \<open>dest_int = dest_V_int o VAL.prj\<close>
+  mk_array_def': \<open>mk_array = VAL.inj o V_array o map VAL.prj\<close>
+  dest_array_def': \<open>dest_array = map VAL.inj o dest_V_array o VAL.prj\<close>
+  by auto
+
+lemma mk_int_inj': \<open>dest_int (mk_int i) = i\<close>
+  unfolding mk_int_def' dest_int_def' by simp
+
+lemma [simp]: \<open>VAL.inj \<circ> VAL.prj = id\<close> by fastforce 
+
+lemma mk_array_inj': \<open>dest_array (mk_array x) = x\<close>
+  unfolding mk_array_def' dest_array_def' by simp
+
+discharge_debt_axiom mk_int_inj : mk_int_inj'
+  and mk_array_inj : mk_array_inj'
+
+print_debt_axiom \<comment> \<open>Good job! No debt axiom is recorded.\<close>
+
+
+end
